Progres on subword property

Coxeter/Bruhat.lean
@@ -23,7 +23,7 @@ variable {W : Type*} [CoxeterGroup W]
 
 inductive le : W → W → Prop
   | rfl (u : W) : le u u
-  | step (u v w : W) (h1 : le u v) (h2 : cs.IsReflection (v⁻¹ * w))
+  | step (u v w : W) (h1 : le u v) (h2 : cs.IsReflection (w * v⁻¹))
       (h3 : cs.length v < cs.length w) : le u w
 
 instance : LE W where
@@ -83,12 +83,106 @@ instance : PartialOrder W where
         have := length_le_of_bruhat_le h3
         grind
 
--- Bjorner--Brenti Corollary 2.2.1 -/
--- theorem reduced_subword_extend {μ ω : List (B W)}
---   (h1 : μ <+ ω) (h2 : cs.IsReduced μ) (h3 : cs.IsReduced ω)
---   (h4 : cs.wordProd μ ≠ cs.wordProd ω) :
+theorem lt_reflection_mul_iff {t : W} (ht : cs.IsReflection t) (w : W)
+  : w < t * w ↔ cs.length w < cs.length (t * w) := by
+  constructor
+  · intro h
+    apply length_lt_of_bruhat_lt
+    exact h
+  · intro h
+    constructor
+    · apply le.step w w (t * w) (le.rfl _)
+      · rw [mul_inv_cancel_right]
+        exact ht
+      · exact h
+    · intro h2
+      rw [←h2] at h
+      grind
+
+theorem reflection_mul_lt_iff {t : W} (ht : cs.IsReflection t) (w : W)
+  : t * w < w ↔ cs.length (t * w) < cs.length w := by
+  have h := lt_reflection_mul_iff ht (t * w)
+  rw [←mul_assoc, ht.mul_self, one_mul] at h
+  exact h
+
+theorem mul_reflection_lt_or_gt (w : W) {t : W} (ht : cs.IsReflection t) :
+  t * w < w ∨ t * w > w := by
+  conv in t * w > w => change w < t * w
+  rw [reflection_mul_lt_iff ht, lt_reflection_mul_iff ht]
+  exact Nat.lt_or_gt_of_ne (ht.length_mul_right_ne w)
+
+def ReducedWord (w : W) := {ω : List (B W) // w = cs.wordProd ω ∧ cs.IsReduced ω}
+
+instance {w : W} : CoeOut (ReducedWord w) (List (B W)) where
+  coe := fun ω => ω.val
+
+/-- Bjorner--Brenti Theorem 2.2.2 (only if) -/
+theorem exists_reduced_subword_of_le (u w : W) (h : u ≤ w) (ω : ReducedWord w) :
+  ∃ μ : ReducedWord u, μ.val <+ ω.val := by
+  revert ω
+  induction h with
+  | rfl =>
+      intro ω
+      exists ω
+  | step v w _ h1 h2 ih =>
+      intro ω
+      let t := w * v⁻¹
+      change cs.IsReflection t at h1
+      have h3 : w = t * v := by simp only [inv_mul_cancel_right, t]
+      have h4 : cs.IsLeftInversion (cs.wordProd ω) t := by
+        constructor
+        · exact h1
+        · rw [←ω.prop.1]
+          nth_rw 1 [h3]
+          rw [←mul_assoc, h1.mul_self, one_mul]
+          exact h2
+      have ⟨i, _, h5⟩ := strong_exchange h4
+      nth_rw 1 [←ω.prop.1, h3, ←mul_assoc, h1.mul_self, one_mul] at h5
+      have ⟨ω', h6, _, _⟩ := exists_reduced_subword (ω.val.eraseIdx i)
+      have ⟨μ, h7⟩ := ih ⟨ω', by grind⟩
+      exists μ
+      calc
+        μ <+ ω' := h7
+        _ <+ ω.val.eraseIdx i := h6
+        _ <+ ω := eraseIdx_sublist _ _
+
+-- open Classical in
+-- Bjorner--Brenti Lemma 2.2.1 -/
+-- theorem reduced_subword_extend {u w : W} (ω : ReducedWord w)
+--   (h1 : u ≠ cs.wordProd ω) (h2 : ∃ (μ : ReducedWord u), μ.val <+ ω.val) :
 --   ∃ (ν : List (B W)), ν <+ ω ∧ cs.IsReduced ν
---     ∧ cs.wordProd ν > cs.wordProd μ ∧ ν.length = μ.length + 1 := by
---   sorry
+--     ∧ cs.wordProd ν > u ∧ ν.length = cs.length u + 1 := by
+--   let P (i : ℕ) := ∃ (μ : ReducedWord u), μ.val <+ ω.val ∧ take i μ.val = take i ω.val
+--   let i := Nat.findGreatest P ω.val.length
+--   have h3 : P i := by
+--     unfold i
+--     apply Nat.findGreatest_spec (zero_le _)
+--     unfold P
+--     simp only [take_zero, and_true]
+--     exact h2
+--   have h4 : ∀ k > i, ¬ P k := by
+--     intro k hk
+--     cases Nat.le_or_ge k ω.val.length with
+--     | inl h => exact Nat.findGreatest_is_greatest hk h
+--     | inr h =>
+--         intro ⟨μ, hμ⟩
+--         have hμ2 : μ.val.length ≤ k := by grind
+--         rw [take_of_length_le hμ2, take_of_length_le h] at hμ
+--         grind
+--   have ⟨μ, h5, h6⟩ := h3
+--   have h7 : i < ω.val.length := by
+--     suffices i ≠ ω.val.length by
+--       have : i ≤ ω.val.length := Nat.findGreatest_le _
+--       grind
+--     intro h
+--     rw [h, take_length] at h6
+--     grind
+--   have h6 : take (i + 1) μ ≠ take (i + 1) ω.val := by grind
+--   let t := cs.wordProd (take i ω) * cs.simple ω.val[i] * (cs.wordProd (take i ω))⁻¹
+--   have ht : cs.IsReflection t := by exists cs.wordProd (take i ω.val), ω.val[i]
+--   cases mul_reflection_lt_or_gt u ht with
+--   | inl h => sorry
+--   | inr h => sorry
+
 
 end Coxeter
